transformations/Class2Relational_TUPLE_SP/theorems/Elements.v
@@ -10,8 +10,6 @@ Require Import core.Model.
 
 From transformations.Class2Relational_TUPLE_SP
   Require
-(*  ClassModelProperties 
-  RelationalModelProperties *)
   C2RTactics
   Class2Relational_TUPLE_SP.
 
@@ -58,7 +56,7 @@ Proof.
   intros cm rm H ; subst.
   intros i n i2 n2 H1 H2 H3.
   simpl.
-  unfold traceTrOnModel.
+  unfold compute_trace.
   rewrite map_flat_map.
   apply List.in_flat_map.
   exists ([AttributeElement
@@ -122,7 +120,7 @@ Proof.
   intros cm rm H ; subst.
   intros i n H.
   simpl.
-  unfold traceTrOnModel. 
+  unfold compute_trace. 
   apply C2RTactics.allModelElements_allTuples in H.
   revert H ; generalize (allTuples Class2Relational_TUPLE_SP cm).
 
